theories/ordinals/Hydra/Hydra_Lemmas.v
@@ -307,7 +307,7 @@ Proof.
 Qed.
 
 Lemma variant_mono_free  {A:Type} {Lt: relation A}{Tr : Transitive Lt}
-      {Wf: well_founded Lt} m {V: Hvariant Wf free m}:
+      {Wf: well_founded Lt} m {V: Hvariant (Lt:=Lt) (Wf:=Wf) free m}:
   forall i h j h', battle free i h j h' -> Lt (m h') (m h).
 Proof.
   induction 1;auto. 
@@ -321,7 +321,7 @@ Proof.
 Qed.
 
 Lemma m_strict_mono  {A:Type} {Lt: relation A}{St: StrictOrder  Lt}
-      {Wf: well_founded Lt} m (V: Hvariant Wf free m){h h':Hydra}:
+      {Wf: well_founded Lt} m (V: @Hvariant _ _ Wf free m){h h':Hydra}:
   h -+->  h' -> Lt (m h') (m h).
  Proof.
       induction 1;auto.
@@ -377,7 +377,7 @@ Qed.
 
 Lemma Hvariant_Termination {A : Type} {lt : relation A}
       (Hwf : well_founded lt) (m : Hydra -> A) :
-  Hvariant Hwf  free m ->  Termination.
+  @Hvariant _ _ Hwf  free m ->  Termination.
 Proof.
   destruct 1.
   intro x; apply Acc_incl with (fun h' h =>  lt (m h') (m h)).
