theories/ordinals/Hydra/Hydra_Theorems.v
@@ -31,20 +31,20 @@ Qed.
 (** ** Termination of free battles 
  *)
 
-Theorem Variant_LT_free_0 :  Hvariant  T1_wf free Hydra_Termination.m.
+Theorem Variant_LT_free_0 :  @Hvariant  _ _ T1_wf free Hydra_Termination.m.
 Proof. split; intros; now apply round_decr. Qed.
 
-Theorem Variant_lt_free:  Hvariant E0.Lt_wf free Hydra_Termination.var.
+Theorem Variant_lt_free:  @Hvariant _ _ E0.Lt_wf free Hydra_Termination.var.
 Proof. split; intros; now apply round_decr. Qed.
 
 
-Theorem Variant_LT_standard : Hvariant T1_wf standard Hydra_Termination.m.
+Theorem Variant_LT_standard : @Hvariant _ _ T1_wf standard Hydra_Termination.m.
 Proof.
  split; intros i h h' H H0; apply round_decr; now exists i.
 Qed.
 
 
-Theorem Variant_lt_standard : Hvariant E0.Lt_wf standard Hydra_Termination.var.
+Theorem Variant_lt_standard : @Hvariant _ _ E0.Lt_wf standard Hydra_Termination.var.
 Proof.
   split; intros i h h' H H0;  apply round_decr; now exists i.
 Qed.
@@ -61,6 +61,8 @@ Print Assumptions Variant_lt_standard.
 
 (** A helper : to do: remove if useless *)
 
+(**  Impossiblity to define a variant bounded by some ordinal less than 
+     [epsilon0] *)
 
 Check Impossibility_free.
 (*
