theories/ordinals/Hydra/Omega2_Small.v
@@ -16,7 +16,7 @@ Section Impossibility_Proof.
 
   Variable m : Hydra -> ON_Omega2.t.
  
-  Context (Hvar : Hvariant (Generic.wf (ON:=Omega2))  free m).
+  Context (Hvar : @Hvariant _ _ (Generic.wf (ON:=Omega2))  free m).
   
   Let big_h := hyd1 (hyd2 head head).
   
